build the fundemental sequence according to the guidelines of Sylvain. Much shorter spec. Remains to show that it exists (which induction principle) and that its lub is the corresponding limit ordinal !!

theories/eps0.v
@@ -62,6 +62,48 @@ Proof. rewrite in_app_iff; simpl; tauto. Qed.
 Fact snoc_assoc X l (x y : X) : l++[x;y] = (l++[x])++[y].
 Proof. now rewrite <- app_assoc. Qed.
 
+Fact list_split {X} (l₁ l₂ r₁ r₂ : list X) :
+    l₁++r₁ = l₂++r₂
+  → ∃m, l₁++m = l₂ ∧ r₁ = m++r₂
+     ∨  l₁ = l₂++m ∧ m++r₁ = r₂.
+Proof.
+  revert l₂; induction l₁ as [ | x l1 IH ]; intros [ | y l2 ]; simpl.
+  + exists []; auto.
+  + intros ->; eauto.
+  + intros <-; eauto.
+  + injection 1; intros (m & [ [] | [] ])%IH <-; subst; eauto.
+Qed.
+
+Fact list_split_cons {X} (l₁ l₂ r₁ r₂ : list X) x :
+    l₁++r₁ = l₂++[x]++r₂
+  → ∃m, l₁++m = l₂ ∧ r₁ = m++[x]++r₂
+     ∨  l₁ = l₂++[x]++m ∧ m++r₁ = r₂.
+Proof.
+  intros (m & [ [H1 H2] | [H1 H2] ])%list_split; subst; eauto.
+  destruct m as [ | y m ]; simpl in H2.
+  + subst; exists []; rewrite !app_nil_r; auto.
+  + inversion H2; subst; exists m; auto.
+Qed. 
+
+Fact list_split_cons2 {X} (l₁ l₂ r₁ r₂ : list X) x y :
+    l₁++[x]++r₁ = l₂++[y]++r₂
+  → l₁ = l₂ ∧ x = y ∧ r₁ = r₂
+  ∨ ∃m, l₁++[x]++m = l₂ ∧ r₁ = m++[y]++r₂
+     ∨  l₁ = l₂++[y]++m ∧ m++[x]++r₁ = r₂.
+Proof.
+  intros (m & [ [H1 H2] | [H1 H2] ])%list_split; subst.
+  + destruct m as [ | z m ]; simpl in H2.
+    * inversion H2; subst y r₂.
+      rewrite app_nil_r; auto.
+    * inversion H2; subst z r₁.
+      right; exists m; auto.
+  + destruct m as [ | z m ]; simpl in H2.
+    * inversion H2; subst y r₂.
+      rewrite app_nil_r; auto.
+    * inversion H2; subst z r₂.
+      right; exists m; auto.
+Qed. 
+
 Section wf_rel_morph.
 
   Variables (X Y : Type) (R : X → X → Prop) (T : Y → Y → Prop)
@@ -716,19 +758,29 @@ Qed.
 Fact E0_lpo_trans' e f : clos_trans E0_lpo e f → E0_lpo e f.
 Proof. induction 1; eauto. Qed.
 
-Definition E0_zero := ω[[]].
-
-Fact E0_zero_lt e : E0_zero = e ∨ E0_zero <E₀ e.
-Proof.
-  destruct e as [ [] ]; [ left | right ]; eauto.
-  repeat constructor.
-Qed.
-
 Definition E0_le e f := e <E₀ f ∨ e = f.
 
 Notation "e '≤E₀' f" := (E0_le e f) (at level 70, format "e  ≤E₀  f").
 
-Fact E0_zero_not_gt e : ¬ e <E₀ E0_zero.
+Fact E0_le_refl e : e ≤E₀ e.
+Proof. now right. Qed.
+
+Fact E0_le_trans : transitive E0_le.
+Proof. intros ? ? ? [] []; subst; red; eauto. Qed.
+
+#[local] Hint Resolve E0_le_refl E0_le_trans : core.
+
+Definition E0_zero := ω[[]].
+
+Notation "0₀" := E0_zero.
+
+Fact E0_zero_le e : 0₀ ≤E₀ e.
+Proof.
+  destruct e as [ [] ]; [ right | left ]; eauto.
+  repeat constructor.
+Qed.
+
+Fact E0_zero_not_gt e : ¬ e <E₀ 0₀.
 Proof.
   destruct e as [ l ].
   intros ?%E0_lt_inv%lex_list_inv.
@@ -766,6 +818,15 @@ Proof.
   apply and_iff_compat_l.
   split; intros H ? ? []%H; split; auto; apply cnf_iff; auto.
 Qed.
+
+Fact cnf_sg e i : cnf e → 0 < i → cnf ω[[(e,i)]].
+Proof.
+  rewrite cnf_fix; split.
+  + repeat constructor.
+  + intros ? ? [[=]|[]]; subst; eauto.
+Qed.
+
+#[local] Hint Resolve cnf_sg : core.
 
 (* We convert the recursor *)
 Fact cnf_rect (P : E0 → Type) :
@@ -920,7 +981,8 @@ Qed.
 Fact E0_one_ge r : r ≠ [] → cnf ω[r] → E0_one ≤E₀ ω[r].
 Proof.
   destruct r as [ | (x,i) r ]; [ easy | intros _ Hr ].
-  destruct (E0_zero_lt x) as [ <- | Hx ].
+  destruct (E0_zero_le x) as [ Hx | <- ].
+  + left; constructor; constructor; now left.
   + destruct i as [ | [ | i ] ].
     * apply cnf_fix, proj2 in Hr.
       destruct (Hr E0_zero 0); auto; lia.
@@ -929,7 +991,6 @@ Proof.
       - now right.
       - left; constructor; constructor 1.
     * left; constructor; constructor; right; lia.
-  + left; constructor; constructor; now left.
 Qed.
 
 Inductive E0_succ_graph : E0 → E0 → Prop :=
@@ -978,7 +1039,7 @@ Definition E0_add e f :=
   | ω[l], ω[m] => ω[wlist_combine E0_lt_sdec l m]
   end.
 
-Fact E0_add_correct : ∀ e f, cnf e → cnf f → cnf (E0_add e f).
+Fact E0_add_cnf : ∀ e f, cnf e → cnf f → cnf (E0_add e f).
 Proof.
   intros [l] [m] (H1 & H2)%cnf_fix (H3 & H4)%cnf_fix; apply cnf_fix.
   split.
@@ -1011,56 +1072,13 @@ Proof.
   + now apply E0_zero_not_gt in H2.
 Qed.
 
-Fact list_split {X} (l₁ l₂ r₁ r₂ : list X) :
-    l₁++r₁ = l₂++r₂
-  → ∃m, l₁++m = l₂ ∧ r₁ = m++r₂
-     ∨  l₁ = l₂++m ∧ m++r₁ = r₂.
-Proof.
-  revert l₂; induction l₁ as [ | x l1 IH ]; intros [ | y l2 ]; simpl.
-  + exists []; auto.
-  + intros ->; eauto.
-  + intros <-; eauto.
-  + injection 1; intros (m & [ [] | [] ])%IH <-; subst; eauto.
-Qed.
-
-Fact list_split_cons {X} (l₁ l₂ r₁ r₂ : list X) x :
-    l₁++r₁ = l₂++[x]++r₂
-  → ∃m, l₁++m = l₂ ∧ r₁ = m++[x]++r₂
-     ∨  l₁ = l₂++[x]++m ∧ m++r₁ = r₂.
-Proof.
-  intros (m & [ [H1 H2] | [H1 H2] ])%list_split; subst; eauto.
-  destruct m as [ | y m ]; simpl in H2.
-  + subst; exists []; rewrite !app_nil_r; auto.
-  + inversion H2; subst; exists m; auto.
-Qed. 
-
-Fact list_split_cons2 {X} (l₁ l₂ r₁ r₂ : list X) x y :
-    l₁++[x]++r₁ = l₂++[y]++r₂
-  → l₁ = l₂ ∧ x = y ∧ r₁ = r₂
-  ∨ ∃m, l₁++[x]++m = l₂ ∧ r₁ = m++[y]++r₂
-     ∨  l₁ = l₂++[y]++m ∧ m++[x]++r₁ = r₂.
-Proof.
-  intros (m & [ [H1 H2] | [H1 H2] ])%list_split; subst.
-  + destruct m as [ | z m ]; simpl in H2.
-    * inversion H2; subst y r₂.
-      rewrite app_nil_r; auto.
-    * inversion H2; subst z r₁.
-      right; exists m; auto.
-  + destruct m as [ | z m ]; simpl in H2.
-    * inversion H2; subst y r₂.
-      rewrite app_nil_r; auto.
-    * inversion H2; subst z r₂.
-      right; exists m; auto.
-Qed. 
-
-
 (* Proof that if cnf u then
    either u is E0_zero                             (limit ordinal)
       or  u is ω[l++[(E0_zero,i)]])                (successor)
       or  u is ω[l++[(e,i)]]) with  E0_zero <E₀ e  (limit ordinal) *)
 
 (** This proof needs much better automation ... *)
-Theorem E0_add_mono u v e : cnf u → cnf v → cnf e → u ≤E₀ v → E0_add u e ≤E₀ E0_add v e.
+Theorem E0_add_mono_left u v e : cnf u → cnf v → cnf e → u ≤E₀ v → E0_add u e ≤E₀ E0_add v e.
 Proof.
   intros Hu Hv He [ H | -> ]; [ | right ]; auto.
   revert u v e Hu Hv He H.
@@ -1185,7 +1203,6 @@ Proof.
         rewrite !wlist_combine_gt_list with (3 := G1); auto.
         simpl app at 2 4.
         rewrite !wlist_combine_lt; eauto.
-        now right.
       - subst l m'.
         rewrite !Forall_app in G1.
         destruct G1 as (G1 & G4 & G3).
@@ -1202,7 +1219,6 @@ Proof.
         rewrite <- !app_assoc.
         rewrite !wlist_combine_gt_list with (3 := G1); auto.
         simpl app at 2 6; rewrite !wlist_combine_lt; auto.
-        right; auto.
   + unfold E0_add.
     destruct (wlist_cut_choice E0_lt_sdec (p++[(x,j)]++m') z)
       as [ G1 
@@ -1235,14 +1251,12 @@ Proof.
         rewrite !wlist_combine_gt_list with (3 := G1); auto.
         simpl app at 2 6.
         rewrite !wlist_combine_eq; auto.
-        right; auto.
     * apply list_split_cons2 in E
         as [ (<- & [=] & <-) | (m & [ (E1 & E2) | (E1 & E2) ]) ].
       - subst x' i'.
         simpl app.
         rewrite !wlist_combine_gt_list; auto.
         rewrite !wlist_combine_lt; auto.
-        right; auto.
       - subst l m'.
         rewrite !Forall_app in G1.
         destruct G1 as (G1 & G4 & G3).
@@ -1256,23 +1270,251 @@ Proof.
         rewrite <- !app_assoc.
         rewrite !wlist_combine_gt_list with (3 := G1); auto.
         simpl app at 2 6; rewrite !wlist_combine_lt; auto.
-        right; auto.
 Qed.
 
-Definition is_lub {X} (R : X → X → Prop) (P : X → Prop) u := ∀v, (∀x, P x → R x v) ↔ R u v.
+Theorem E0_add_incr e f : cnf e → cnf f → E0_zero <E₀ f → e <E₀ E0_add e f.
+Proof.
+  revert e f.
+  intros [l] [[| (y,j) m]] He Hf.
+  1: now intros ?%E0_lt_irrefl.
+  intros _.
+  unfold E0_add.
+  destruct (wlist_cut_choice E0_lt_sdec l y)
+      as [ G1 
+       | [ (i & l' & r & E & G1) 
+       |   (x & i & l' & r & E & G1 & G2) ] ].
+  + rewrite wlist_combine_spec1; auto.
+    constructor; simpl.
+    rewrite <- (app_nil_r l) at 1. 
+    apply lex_list_app_head; constructor 1.
+  + subst l.
+    rewrite wlist_combine_spec2; auto.
+    constructor; simpl.
+    apply lex_list_app_head; constructor 2.
+    right.
+    apply cnf_fix, proj2 in Hf.
+    destruct (Hf y j); auto; lia.
+  + subst l.
+    rewrite wlist_combine_spec3; auto.
+    constructor; simpl.
+    apply lex_list_app_head; constructor 2.
+    now left.
+Qed.
 
-(** The lub is preserved *)
+Theorem E0_add_mono_right e u v : cnf e → cnf u → cnf v → u <E₀ v → E0_add e u <E₀ E0_add e v.
+Proof.
+  revert e u v.
+  intros [l] [m] [[|(z,h) k]] Hl Hm Hk.
+  1: intros []%E0_zero_not_gt.
+  destruct m as [ | yj m ].
+  1: intros; apply E0_add_incr; eauto.
+  intros [ (y,j) [ Hyz | (<- & Hjh) ]%lex2_inv | Hmk ]%E0_lt_inv%lex_list_inv; constructor.
+  + unfold E0_add.
+    destruct (wlist_cut_choice E0_lt_sdec l z)
+      as [ G1 
+       | [ (i & l' & r' & E & G1) 
+       |   (x & i & l' & r' & E & G1 & G2) ] ].
+    * rewrite !wlist_combine_spec1; auto.
+      2: revert G1; apply Forall_impl; eauto.
+      apply lex_list_app_head; constructor 2; now left.
+    * subst l.
+      simpl app.
+      rewrite !wlist_combine_gt_list; auto.
+      2: revert G1; apply Forall_impl; eauto.
+      apply lex_list_app_head.
+      rewrite wlist_combine_gt; auto.
+      rewrite wlist_combine_eq; auto.
+      constructor 2; right.
+      apply cnf_fix, proj2 in Hk.
+      destruct (Hk z h); eauto; lia.
+    * subst l.
+      simpl app.
+      rewrite !wlist_combine_gt_list; auto.
+      2: revert G1; apply Forall_impl; eauto.
+      apply lex_list_app_head.
+      rewrite wlist_combine_lt with (y := z); auto.
+      destruct (wlist_combine_choice E0_lt_sdec)
+        with (x := x) (i := i) (y := y) (j := j) (l := r') (m := m)
+        as (a & b & c & -> & H); auto.
+      constructor 2; left.
+      destruct H as [ (_ & <- & _) | [ (_& <- & _) | (_ & -> & _)] ]; auto.
+  + destruct (wlist_cut_choice E0_lt_sdec l y)
+      as [ G1 
+       | [ (i & l' & r' & E & G1) 
+       |   (x & i & l' & r' & E & G1 & G2) ] ].
+    * rewrite !wlist_combine_spec1; auto.
+      apply lex_list_app_head; constructor 2; now right.
+    * subst l.
+      rewrite !wlist_combine_spec2; auto.
+      apply lex_list_app_head; constructor 2; right; lia.
+    * subst.
+      rewrite !wlist_combine_spec3; auto.
+      apply lex_list_app_head; constructor 2; now right.
+  + now apply lex_list_app_head.
+Qed.
+
+Definition E0_is_succ e := ∃f, e = E0_succ f.
+Definition E0_is_limit e := e ≠ 0₀ ∧ ¬ ∃f, e = E0_succ f.
+
+Inductive E0_decomp : E0 → Type :=
+  | E0_decomp_zero : E0_decomp 0₀
+  | E0_decomp_succ e : cnf e → E0_decomp (E0_succ e)
+  | E0_decomp_limit g e : e <> 0₀ → cnf g → cnf e → E0_decomp (E0_add g ω[[(e,1)]]).
+
+Lemma E0_decomp_compute e : cnf e → E0_decomp e.
+Proof.
+  induction 1 as [ m H1 H2 H3 _ ] using cnf_rect.
+  destruct m as [ | m (e,i) _ ] using rev_rect.
+  + constructor 1.
+  + destruct i as [ | i ].
+    1: destruct (@lt_irrefl 0); eauto.
+    destruct e as [[ | yj e ]].
+    * destruct i as [ | i ].
+      - replace ω[m++[(ω[[]],1)]]
+          with (E0_succ ω[m]).
+        ++ constructor.
+           apply cnf_fix; repeat split; eauto.
+           rewrite map_app in H1.
+           now apply ordered_app_head in H1.
+        ++ apply E0_succ_graph_fun with (1 := E0_succ_spec _).
+           destruct m as [ | m (x,i) _ ] using rev_rect.
+           ** constructor.
+           ** rewrite <- app_assoc.
+              constructor.
+              intros ->.
+              rewrite !map_app, <- app_assoc in H1.
+              now apply ordered_app_tail, ordered_inv,
+                    ordered_from_inv, proj1, E0_lt_irrefl in H1.
+      - replace ω[m++[(ω[[]],S (S i))]]
+          with (E0_succ ω[m++[(0₀,S i)]]).
+        ++ constructor 2.
+           apply cnf_fix; split.
+           ** rewrite map_app in H1 |- *; auto.
+           ** intros ? ? [|[[=]|[]]]%in_app_iff; split; subst; eauto; lia.
+        ++ apply E0_succ_graph_fun with (1 := E0_succ_spec _).
+           constructor 2.
+    * destruct i as [ | i ].
+      - replace ω[m++[(ω[yj::e],1)]]
+          with (E0_add ω[m] ω[[(ω[yj::e],1)]]).
+        ++ constructor 3; easy || eauto.
+           apply cnf_fix; repeat split; eauto.
+           rewrite map_app in H1.
+           now apply ordered_app_head in H1.
+        ++ unfold E0_add.
+           rewrite wlist_combine_spec1; eauto.
+           rewrite map_app in H1; simpl in H1.
+           apply ordered_snoc_iff, proj2 in H1; auto.
+           apply Forall_forall.
+           now intros (f,i) H; apply H1, in_map.
+      - replace ω[m++[(ω[yj::e], S (S i))]]
+          with (E0_add ω[m++[(ω[yj::e],S i)]] ω[[(ω[yj::e],1)]]).
+        ++ constructor 3; easy || eauto.
+           apply cnf_fix; split.
+           ** rewrite map_app in H1 |- *; auto.
+           ** intros f j [|[[=]|[]]]%in_app_iff; split; subst; eauto; lia.
+        ++ unfold E0_add.
+           rewrite <- (app_nil_r (_++[_])), <- app_assoc.
+           rewrite wlist_combine_spec2; auto.
+           ** rewrite app_nil_r; do 4 f_equal; lia.
+           ** rewrite map_app in H1; simpl in H1. 
+              apply ordered_snoc_iff, proj2 in H1; auto.
+              apply Forall_forall.
+              intros [] ?; now apply H1, in_map.
+Qed.
+
+Inductive E0_fseq_gr : E0 → (nat → E0) → Prop :=
+  | E0_fseq_gr_0 g b   : cnf g
+                       → cnf b
+                       → E0_fseq_gr (E0_add g ω[[(E0_succ b,1)]]) (λ n, E0_add g ω[[(b,1+n)]])
+  | E0_fseq_gr_1 g b r : cnf g
+                       → cnf b
+                       → E0_fseq_gr b r
+                       → E0_fseq_gr (E0_add g ω[[(b,1)]]) (λ n, E0_add g ω[[(r n,1)]]).
+
+(** WF Induction on e st cnf e *)
+Theorem E0_fseq_pwc e : cnf e → E0_is_limit e → sig (E0_fseq_gr e).
+Proof.
+(*
+  induction e as [ e IHe ] using (well_founded_induction_type E0_lt_wf).
+  induction 1 as [ m H1 H2 H3 IH ] using cnf_rect; intros (G1 & G2).
+  destruct 
+*)
+Admitted.
+
+Definition E0_fseq {e} (h : cnf e) (l : E0_is_limit e) := proj1_sig (@E0_fseq_pwc e h l).
+Fact E0_fseq_spec e h l : E0_fseq_gr e (@E0_fseq e h l).
+Proof. apply (proj2_sig _). Qed.
+
+Fact E0_fseq_gr_cnf e r : E0_fseq_gr e r → ∀n, cnf (r n).
+Proof.
+  induction 1; intro.
+  + apply E0_add_cnf; auto.
+    apply cnf_sg; auto; lia.
+  + apply E0_add_cnf; auto.
+Qed. 
+
+(** The fundemental sequence is correct *)
+Fact E0_fseq_cnf e h l n : cnf (@E0_fseq e h l n).
+Proof. generalize (E0_fseq_spec h l) n; apply E0_fseq_gr_cnf. Qed.
+
+#[local] Hint Resolve E0_fseq_gr_cnf E0_fseq_cnf : core.
+
+(** The fundemental sequence is increasing *)
+Fact E0_fseq_incr e h l : ∀ n m, n < m → @E0_fseq e h l n <E₀ E0_fseq h l m.
+Proof.
+  generalize (E0_fseq h l) (E0_fseq_spec h l); clear l.
+  induction 1; intros.
+  + apply E0_add_mono_right; auto.
+    1,2: apply cnf_sg; auto; lia.
+    constructor; constructor 2; right; lia.
+  + apply E0_add_mono_right; auto.
+    1,2: apply cnf_sg; eauto.
+    constructor; constructor 2; left; eauto.
+Qed.
+
+(** We need to show that n E0_fseq e h l n *)
+
+Definition is_lub {X} (R : X → X → Prop) (P : X → Prop) u := ∀v, (∀x, P x → R x v) ↔ R u v.
+Definition dwnwc {X} (R : X → X → Prop) (P : X → Prop) x := ∃y, R x y ∧ P y.
+
+Fact is_lub_dwnwc P u : is_lub E0_le P u → is_lub E0_le (dwnwc E0_le P) u.
+Proof.
+  intros H v; red in H; split.
+  + intros G.
+    rewrite <- H.
+    intros x Hx; apply G; exists x; split; auto.
+  + intros Hu x (e & He & G).
+    rewrite <- H in Hu.
+    apply E0_le_trans with (1 := He); auto.
+Qed.
+
+(** The lub is preserved; for this we need the fundemental sequence *)
 Theorem E0_add_lub P u v : 
      (∀e, P e → cnf e)
    → cnf u
    → cnf v
-   → is_lub E0_le P u
-   → is_lub E0_le (λ x, ∃e, P e ∧ x = E0_add e v) (E0_add u v).
+   → is_lub E0_le P v
+   → is_lub E0_le (λ x, ∃e, P e ∧ x = E0_add u e) (E0_add u v).
+Proof.
+  intros H1 H2 H3 H4%is_lub_dwnwc f; split.
+  + intros H.
+    assert (H' : ∀e, P e → E0_add u e ≤E₀ f).
+    1:{ intros e He; apply H; eauto. }
+    clear H.
+    (* if v is zero
+       if v is succ
+       if v is limit w[l++(e,i)] with 0₀ < e
+       then w[l++(e,i-1)++k] in dwnwc E0_le P (otherwise v is not upper bound) *)
+    admit.
+  + intros H x (e & He & ->).
+    apply E0_le_trans with (2 := H).
+    assert (e ≤E₀ v) as [ G | ].
+    1: apply H4; try red; auto.
+    * left; apply E0_add_mono_right; eauto.
+    * subst; now right.
+Admitted.
 
-(** Then show that 
-      E0_add e E0_zero = e
-  and E0_add e E0_one = E0_succ e 
-    Show also the preservation of lubs *)
+    exists  *)
 
 (** ε₀ is the sub-type of E0 composed of trees in nested lexigraphic order *)
 
